@prefix cc:    <http://creativecommons.org/ns#> .
@prefix owl:   <http://www.w3.org/2002/07/owl#> .
@prefix rdf:   <http://www.w3.org/1999/02/22-rdf-syntax-ns#> .
@prefix rdfs:  <http://www.w3.org/2000/01/rdf-schema#> .

<http://web.resource.org/cc/License>
        owl:equivalentClass  cc:License .

cc:legalcode  rdf:type  rdf:Property ;
        rdfs:domain  cc:License ;
        rdfs:range   rdfs:Resource .

cc:jurisdiction  rdf:type  rdf:Property ;
        rdfs:domain  cc:License ;
        rdfs:label   "jurisdiction"@en-US ;
        rdfs:range   cc:Jurisdiction .

<http://web.resource.org/cc/prohibits>
        owl:equivalentProperty  cc:prohibits .

<http://web.resource.org/cc/CommercialUse>
        owl:equivalentClass  cc:CommercialUse .

cc:useGuidelines  rdf:type  rdf:Property ;
        rdfs:range          rdfs:Resource ;
        rdfs:subPropertyOf  <http://purl.org/dc/terms/relation> ;
        rdfs:domain         cc:Work .

<http://web.resource.org/cc/permits>
        owl:equivalentProperty  cc:permits .

cc:LesserCopyleft  rdf:type  cc:Requirement ;
        rdfs:label    "Lesser Copyleft"@en-US ;
        rdfs:comment  "derivative works must\n\t\t    be licensed under specified terms, with at least\n\t\t    the same conditions as the original work;\n\t\t    combinations with the work may be licensed under\n\t\t    different terms"@en-US .

<http://web.resource.org/cc/Permission>
        owl:equivalentClass  cc:Permission .

<http://web.resource.org/cc/Attribution>
        owl:equivalentClass  cc:Attribution .

<http://web.resource.org/cc/Reproduction>
        owl:equivalentClass  cc:Reproduction .

<http://web.resource.org/cc/Work>
        owl:equivalentClass  cc:Work .

<http://web.resource.org/cc/Requirement>
        owl:equivalentClass  cc:Requirement .

<http://web.resource.org/cc/SourceCode>
        owl:equivalentClass  cc:SourceCode .

cc:attributionURL  rdf:type  rdf:Property ;
        rdfs:domain  cc:Work ;
        rdfs:range   rdfs:Resource .

cc:morePermissions  rdf:type  rdf:Property ;
        rdfs:range          rdfs:Resource ;
        rdfs:subPropertyOf  <http://purl.org/dc/terms/relation> ;
        rdfs:domain         cc:Work .

<http://web.resource.org/cc/ShareAlike>
        owl:equivalentClass  cc:ShareAlike .

<http://web.resource.org/cc/Prohibition>
        owl:equivalentClass  cc:Prohibition .

cc:attributionName  rdf:type  rdf:Property ;
        rdfs:domain  cc:Work ;
        rdfs:range   rdfs:Literal .

cc:HighIncomeNationUse
        rdf:type      cc:Prohibition ;
        rdfs:label    "High Income Nation Use"@en-US ;
        rdfs:comment  "use in a\n\t\t    non-developing country"@en-US .

<http://web.resource.org/cc/Distribution>
        owl:equivalentClass  cc:Distribution .

<http://web.resource.org/cc/requires>
        owl:equivalentProperty  cc:requires .

<http://web.resource.org/cc/Notice>
        owl:equivalentClass  cc:Notice .

<http://web.resource.org/cc/DerivativeWorks>
        owl:equivalentClass  cc:DerivativeWorks .

cc:Sharing  rdf:type  cc:Permission ;
        rdfs:label    "Sharing"@en-US ;
        rdfs:comment  "permits commercial\n\t\t    derivatives, but only non-commercial\n\t\t    distribution"@en-US .

cc:Copyleft  rdf:type  cc:Requirement ;
        rdfs:label    "Copyleft"@en-US ;
        rdfs:comment  "derivative and\n\t\t    combined works must be licensed under specified\n\t\t    terms, similar to those on the original\n\t\t    work"@en-US .

cc:deprecatedOn  rdf:type  rdf:Property ;
        rdfs:domain  cc:License ;
        rdfs:label   "deprecated\n\t\t  on"@en-US ;
        rdfs:range   <http://www.w3.org/2001/XMLSchema-datatypes#date> .

<http://web.resource.org/cc/license>
        owl:equivalentProperty  cc:license .

cc:Permission  rdf:type  rdfs:Class ;
        rdfs:label    "Permission"@en-US ;
        rdfs:comment  "an action that may or\n\t\t    may not be allowed or desired"@en-US .

cc:SourceCode  rdf:type  cc:Requirement ;
        rdfs:label    "Source Code"@en-US ;
        rdfs:comment  "source code (the\n\t\t    preferred form for making modifications) must be\n\t\t    provided when exercising some rights granted by\n\t\t    the license."@en-US .

cc:permits  rdf:type  rdf:Property ;
        rdfs:domain  cc:License ;
        rdfs:label   "permits"@en-US ;
        rdfs:range   cc:Permission .

cc:ShareAlike  rdf:type  cc:Requirement ;
        rdfs:label    "Share Alike"@en-US ;
        rdfs:comment  "derivative works be\n\t\t    licensed under the same terms or compatible terms\n\t\t    as the original work"@en-US .

cc:Notice  rdf:type   cc:Requirement ;
        rdfs:label    "Notice"@en-US ;
        rdfs:comment  "copyright and license\n\t\t    notices be kept intact"@en-US .

cc:Jurisdiction  rdf:type  rdfs:Class ;
        rdfs:label    "Jurisdiction"@en-US ;
        rdfs:comment  "the legal jurisdiction\n\t\t    of a license"@en-US .

cc:DerivativeWorks  rdf:type  cc:Permission ;
        rdfs:label    "Derivative Works"@en-US ;
        rdfs:comment  "distribution of\n\t\t    derivative works"@en-US .

cc:Work  rdf:type     rdfs:Class ;
        rdfs:label    "Work"@en-US ;
        rdfs:comment  "a potentially\n\t\t    copyrightable work"@en-US .

cc:Reproduction  rdf:type  cc:Permission ;
        rdfs:label    "Reproduction"@en-US ;
        rdfs:comment  "making multiple\n\t\t    copies"@en-US .

cc:Distribution  rdf:type  cc:Permission ;
        rdfs:label    "Distribution"@en-US ;
        rdfs:comment  "distribution, public\n\t\t    display, and publicly performance"@en-US .

cc:requires  rdf:type  rdf:Property ;
        rdfs:domain  cc:License ;
        rdfs:label   "requires"@en-US ;
        rdfs:range   cc:Requirement .

cc:CommercialUse  rdf:type  cc:Prohibition ;
        rdfs:label    "Commercial Use"@en-US ;
        rdfs:comment  "exercising rights for\n\t\t    commercial purposes"@en-US .

cc:prohibits  rdf:type  rdf:Property ;
        rdfs:domain  cc:License ;
        rdfs:label   "prohibits"@en-US ;
        rdfs:range   cc:Prohibition .

cc:Requirement  rdf:type  rdfs:Class ;
        rdfs:label    "Requirement"@en-US ;
        rdfs:comment  "an action that may or\n\t\t    may not be requested of you"@en-US .

cc:Prohibition  rdf:type  rdfs:Class ;
        rdfs:label    "Prohibition"@en-US ;
        rdfs:comment  "something you may be\n\t\t    asked not to do"@en-US .

cc:License  rdf:type     rdfs:Class ;
        rdfs:label       "License"@en-US ;
        rdfs:comment     "a set of\n\t\t    requests/permissions to users of a Work, e.g. a\n\t\t    copyright license, the public domain, information\n\t\t    for distributors"@en-US ;
        rdfs:subClassOf  <http://purl.org/dc/terms/LicenseDocument> .

cc:license  rdf:type        rdf:Property ;
        rdfs:range          cc:License ;
        rdfs:domain         cc:Work ;
        owl:sameAs          <http://www.w3.org/1999/xhtml/vocab#license> ;
        rdfs:subPropertyOf  <http://purl.org/dc/terms/license> ;
        rdfs:label          "has\n\t\t  license"@en-US .

cc:Attribution  rdf:type  cc:Requirement ;
        rdfs:label    "Attribution"@en-US ;
        rdfs:comment  "credit be given to\n\t\t    copyright holder and/or author"@en-US .
